\loesung{

\textit{TO DO}

\subsection*{Solution}

\paragraph{Step 1. Compute the mean term.}
\[
f_\emptyset
=\frac{1}{27}\sum_{x_1,x_2,x_3\in\{0,\frac12,1\}}
   \bigl(4x_1 + 2x_2x_3\bigr)
= \underbrace{\frac{1}{3}\cdot4\cdot\frac{1}{2}}_{=\E[4X_1]} \;+\;
  \underbrace{\Bigl(\frac{1}{3}\Bigr)^{2}\!2}_{=\E[2X_2X_3]}
=1 + \tfrac{2}{9} = \tfrac{11}{9}.
\]

\paragraph{Step 2. First‐order terms.}
\[
f_1(x_1)
=\E[f\mid X_1=x_1] - f_\emptyset
= \bigl(4x_1 + \E[2X_2X_3]\bigr) - \tfrac{11}{9}
=4x_1 + \tfrac{2}{9} - \tfrac{11}{9}
=4x_1 - 1.
\]
By symmetry and since $f$ depends only on $x_2x_3$, one finds
\[
f_2(x_2)=0,\qquad f_3(x_3)=0.
\]

\paragraph{Step 3. Second‐order terms.}
For $\{2,3\}$,
\[
f_{23}(x_2,x_3)
=\E[f\mid X_2=x_2,X_3=x_3]
- f_\emptyset - f_2(x_2)-f_3(x_3)
= 4\,\E[X_1] +2x_2x_3 - \tfrac{11}{9}
= \tfrac{4}{2} +2x_2x_3 - \tfrac{11}{9}
=2x_2x_3 - \tfrac{1}{9}.
\]
All other pairs $\{1,2\}$ and $\{1,3\}$ vanish because once you subtract
$f_\emptyset$ and $f_1$, the remaining dependence is zero.

\paragraph{Step 4. Third‐order term.}
\[
f_{123}(x_1,x_2,x_3)
= f(x_1,x_2,x_3)
- \sum_{A\subsetneq\{1,2,3\}} f_A(x_A)
= 4x_1+2x_2x_3
- \bigl(\tfrac{11}{9} + (4x_1-1) + (2x_2x_3-\tfrac{1}{9})\bigr)
=0.
\]

\paragraph{Step 5. Orthogonality check.}
Define the empirical inner product 
\(\langle u,v\rangle = \tfrac1{27}\sum_{x}u(x)\,v(x)\).  Then
\[
\langle f_1, f_{23}\rangle
=\tfrac1{27}\sum_{x_1,x_2,x_3}(4x_1-1)\,(2x_2x_3-\tfrac{1}{9})
= \bigl(\tfrac1{3}\sum(4x_1-1)\bigr)
  \bigl(\tfrac1{3^2}\sum(2x_2x_3-\tfrac19)\bigr)
=0\cdot0=0,
\]
and similarly each distinct pair of nonzero components is orthogonal.
\hfill\(\Box\)

}